src/Bundle.dfy
@@ -1,2 +1,4 @@
 include "Disks/BlockDisk.dfy"
+include "Disks/ZonedDisk.dfy"
+
 include "Refinements/BlockDiskRefinesItself.dfy"
